theories/ub_logic/cf_hashmap.v
@@ -1,0 +1,437 @@
+From clutch.ub_logic Require Export ub_clutch hash lib.map lib.array cf_hash.
+From stdpp Require Import gmap.
+
+Import Hierarchy.
+
+Section coll_free_hashmap.
+
+  Context `{!ub_clutchGS Σ}.
+
+  (*
+
+     A module implementing a "collision-free" hashmap with constant amortized
+     insertion error and 0 lookup error. As in the hash function, we keep track
+     of a threshold R, a current hashmap size S such that (S < R) and total
+     size of hashmap VS. Insertions to this map are done through the use of a
+     collision free hash function to ensure that no collisions happen.
+  *)
+
+  Variable init_val_size : nat.
+  Variable init_r : nat.
+
+
+  Definition insert_elem : val :=
+    λ: "l" "hf" "s" "r" "val_size" "v",
+      let: "off" := "hf" "v" in
+      let: "w" := !("l" +ₗ "off") in
+      if: "w" = #() then
+        ("l" +ₗ "off") <- "v" ;;
+        "s" <- !"s" + #1 ;;
+         if: !"s" = !"r" then
+           let: "l'" := array_resize "l" !"val_size" !"val_size" in
+           "r" <- #2 * !"r";;
+           "val_size" <- #2 * !"val_size";;
+           "l'"
+         else "l"
+      else "l".
+
+
+  Definition filter_units (vs : list val) :=
+    filter (λ v, ¬(v = #())) vs.
+
+
+  Lemma list_filter_insert_True {A : Type} (P : A -> Prop) (H : ∀ x : A, Decision (P x))
+                                (l : list A) (i : nat) (v w : A) :
+    i < length l ->
+    l !! i = Some w ->
+    ¬ (P w) ->
+    (P v) ->
+    filter P (<[i:=v]> l) ≡ₚ  (cons v (filter P l)).
+  Proof.
+    revert i.
+    induction l; intros i Hlen Hi Hw Hv; apply INR_lt in Hlen.
+    - simpl in Hlen.
+      inversion Hlen.
+    - destruct i.
+      + simpl.
+        simpl in Hi; inversion Hi; simplify_eq.
+        do 2 rewrite filter_cons.
+        rewrite decide_True; auto.
+        rewrite decide_False; auto.
+      + simpl.
+        do 2 rewrite filter_cons.
+        destruct (decide (P a)).
+        * rewrite IHl; auto.
+          ** apply Permutation_swap.
+          ** simpl in Hlen.
+             apply lt_INR. lia.
+        * apply IHl; auto.
+          simpl in Hlen.
+          apply lt_INR. lia.
+  Qed.
+
+
+
+  Definition cf_hashmap_raw (l : loc) (ns : gset nat) f (vs s r : loc) : iProp Σ :=
+    ∃ (vsval sval rval : nat) (m : gmap nat nat) (img : list val),
+      (* The reserve of error credits *)
+        vs ↦ #vsval ∗ s ↦ #sval ∗ r ↦ #rval ∗
+        l ↦∗ img ∗
+        ⌜ 0 < vsval ⌝ ∗
+        ⌜ sval < rval ⌝ ∗
+        ⌜ length img = vsval ⌝ ∗
+      (cf_hashfun_raw init_val_size init_r f m vsval sval rval ) ∗
+      ⌜ (filter_units img) ≡ₚ (λ b, LitV (LitInt (Z.of_nat b))) <$> (elements ns) ⌝ ∗
+      ⌜ forall (i v : nat), m !! v = Some i <-> img !! i = Some #v ⌝ ∗
+      ⌜ forall (i : nat), (i < vsval) ->
+                    i ∉ (@map_img _ _ _ _ (gset nat) _ _ _ m) ->
+                    img !! i = Some #() ⌝ ∗
+      ⌜ dom m = ns ⌝.
+
+
+  Lemma wp_hm_insert E l ns f (vs s r : loc) (n : nat) :
+    {{{ cf_hashmap_raw l ns f vs s r ∗
+          € (nnreal_div (nnreal_nat (3 * init_r)) (nnreal_nat(4 * init_val_size))) }}}
+      insert_elem #l f #s #r #vs #n  @ E
+    {{{ l', RET #l';
+          cf_hashmap_raw l' (ns ∪ {[n]}) f vs s r }}}.
+  Proof.
+    iIntros (Φ) "(Htable & Herr) HΦ".
+    iDestruct "Htable" as (vsval sval rval m img)
+                            " (Hvs & Hs & Hr & Hl & %Hvspos & %Hineq & %Hlen & Hhash & %Hperm & %HimgN & %HimgU & %Hdom)".
+    (*
+    iDestruct "Hhash" as (hm vs' s' r' ε)
+                           "(Herr2 & Hvs' & Hs' & Hr' & %Hvspos' & Hratio & -> & Hmap & %Hlsr & %Hlen & Htot_err & %Hcf)".
+    *)
+    assert (#(sval + 1)%nat = #(sval + 1)) as Hsval.
+    {
+      do 2 f_equal. lia.
+    }
+    rewrite /insert_elem.
+    wp_pures.
+    destruct (m !! n) as [v |] eqn:Hlu.
+    - wp_apply (wp_lookup_no_coll with "[Hhash]"); eauto.
+      iIntros (?) "(-> & Hhf)".
+      wp_pures.
+      wp_apply (wp_load_offset with "[Hl //]").
+      { by apply HimgN.  }
+      iIntros "Hl".
+      wp_pures.
+      iApply "HΦ".
+      iModIntro.
+      rewrite /cf_hashmap_raw.
+      iExists vsval, sval, rval, m, img.
+      rewrite /cf_hashfun_raw.
+      iDestruct "Hhf" as (?????) "(?&?&?&?&?&?&?&?&?&?&?& %Hprf)".
+      iFrame.
+      (* TODO: Notation *)
+      iSplitL "Hl"; [done| ].
+      iSplit; [done|].
+      iSplit; [iExists _,_,_,_,_; by iFrame |].
+      iPureIntro.
+      destruct Hprf as (Hcf & Himg). split.
+      + assert ((ns ∪ {[n]}) = ns) as ->; auto.
+        assert (n ∈ ns); [ | set_solver].
+        rewrite -Hdom.
+        by apply elem_of_dom.
+      + rewrite Hdom.
+        assert (n ∈ ns); [ | set_solver].
+        rewrite -Hdom.
+        by apply elem_of_dom.
+    - assert ((sval + 1 < rval)%nat \/ (sval + 1 = rval)%nat) as [Hleq | Heq].
+      {
+        apply INR_lt in Hineq.
+        inversion Hineq.
+        - right. lia.
+        - left. lia.
+      }
+      + wp_apply (wp_insert_no_coll _ _ _ _ _ vsval sval rval with "[$Hhash $Herr]"); eauto.
+        iIntros (k) "(%Hklt & %Hkimg & Hhash)".
+        wp_pures.
+        wp_apply (wp_load_offset with "[Hl //]"); auto.
+        iIntros "Hl".
+        wp_pures.
+        wp_apply (wp_store_offset with "[Hl //]").
+        { apply lookup_lt_is_Some_2.
+          rewrite Hlen.
+          by apply INR_lt.
+        }
+        iIntros "Hl".
+        wp_pures.
+        wp_load.
+        wp_store.
+        wp_load.
+        wp_load.
+        wp_pures.
+        rewrite bool_decide_eq_false_2; last first.
+        {
+          intro H.
+          inversion H.
+          lia.
+        }
+        wp_pures.
+        iApply "HΦ".
+        iModIntro.
+        rewrite /cf_hashmap_raw.
+        iExists _, (sval + 1)%nat, _, _, (<[k:=#n]> img).
+        rewrite /cf_hashfun_raw.
+        iDestruct "Hhash" as (?????) "(?&?&?&?&?&?&?&?&?&?&?& %Hprf)".
+        iFrame.
+        iSplitL "Hs"; [by rewrite Hsval |].
+        iSplitL "Hl"; [done | ].
+        iSplit.
+        { iPureIntro.
+          rewrite insert_length //.
+        }
+        iSplit.
+        { iExists _,_,_,_,_.
+          iFrame.
+          iSplit; [ done |].
+          iSplit; [| done].
+          iPureIntro.
+          by apply lt_INR.
+        }
+        iPureIntro.
+        destruct Hprf as (Hcf & Himg). split; [| split; [|split]].
+        * rewrite /filter_units /=.
+          rewrite list_filter_insert_True; auto.
+          2:{ rewrite Hlen //. }
+          rewrite union_comm.
+          rewrite elements_union_singleton /=; last first.
+          {
+            intros H.
+            assert (#n ∈ filter_units img) as H2.
+            {
+              rewrite Hperm.
+              apply (elem_of_list_fmap).
+              eexists; split; eauto.
+              set_solver.
+            }
+            rewrite /filter_units in H2.
+            apply elem_of_list_filter in H2 as (H3 & H4).
+            apply elem_of_list_lookup_1 in H4 as (i & Hi).
+            apply HimgN in Hi. simplify_eq.
+          }
+          by apply perm_skip.
+        * intros i v; split; intros H.
+          ** destruct (decide (k = i)) as [-> | Hneqki].
+             *** rewrite list_lookup_insert; [ | apply INR_lt; rewrite Hlen // ].
+                 destruct (decide (n = v)) as [-> | Hneqnv]; auto.
+                 rewrite lookup_insert_ne in H; auto.
+                 exfalso. apply Hkimg.
+                 by eapply elem_of_map_img_2.
+             *** rewrite list_lookup_insert_ne; auto.
+                 apply HimgN.
+                 destruct (decide (n = v)) as [-> | Hneqnv]; auto.
+                 **** rewrite lookup_insert in H.
+                      inversion H; done.
+                 **** rewrite lookup_insert_ne in H; auto.
+          ** destruct (decide (n = v)) as [-> | Hneqnv].
+             *** rewrite lookup_insert.
+                 destruct (decide (k = i)) as [-> | Hneqki]; auto.
+                 rewrite list_lookup_insert_ne in H; auto.
+                 exfalso. apply Hkimg.
+                 set_solver.
+             *** rewrite lookup_insert_ne; auto.
+                 apply HimgN.
+                 destruct (decide (k = i)) as [-> | Hneqki]; auto.
+                 **** rewrite list_lookup_insert in H; [inversion H; simplify_eq | ].
+                      rewrite Hlen. apply INR_lt; auto.
+                 **** rewrite list_lookup_insert_ne in H; auto.
+        * intros i Hi Hiimg.
+          destruct (decide (k = i)) as [-> | Hneqki].
+          ** exfalso.
+             apply Hiimg.
+             eapply elem_of_map_img.
+             exists n. rewrite lookup_insert //.
+          ** rewrite list_lookup_insert_ne; eauto.
+             apply HimgU; auto.
+             intro Him.
+             apply Hiimg.
+             rewrite map_img_insert_notin; auto.
+             set_solver.
+
+        * rewrite dom_insert_L.
+          rewrite Hdom. set_solver.
+
+      + iPoseProof (cf_hashfun_bounded_prf with "[Hhash //]") as "(%Hprf_pre & Hhash)".
+        wp_apply (wp_insert_no_coll_resize _ _ _ _ _ vsval sval rval with "[$Hhash $Herr]"); eauto.
+        iIntros (k) "(%Hklt & %Hkimg & Hhash)".
+        wp_pures.
+        wp_apply (wp_load_offset with "[Hl //]"); auto.
+        iIntros "Hl".
+        wp_pures.
+        wp_apply (wp_store_offset with "[Hl //]").
+        { apply lookup_lt_is_Some_2.
+          rewrite Hlen.
+          by apply INR_lt.
+        }
+        iIntros "Hl".
+        wp_pures.
+        wp_load.
+        wp_store.
+        wp_load.
+        wp_load.
+        wp_pures.
+        rewrite bool_decide_eq_true_2; last first.
+        { do 2 f_equal. lia. }
+        wp_pures.
+        wp_load.
+        wp_load.
+        wp_bind (array_resize _ _ _).
+        rewrite -Hsval.
+        wp_apply (wp_array_resize _ l _ (<[k:=#n]> img) _ _ with "[Hl]"); auto; try lia.
+        { rewrite insert_length. lia. }
+        { by apply INR_lt. }
+        { by apply INR_lt. }
+        iIntros (l') "(Hl & Hl')".
+        wp_pures.
+        wp_load.
+        wp_store.
+        wp_load.
+        wp_store.
+        iApply "HΦ".
+        iModIntro.
+        replace (#(2 * rval)) with (#(2 * rval)%nat); last first.
+        { do 2 f_equal. lia. }
+        replace (#(2 * vsval)) with (#(2 * vsval)%nat); last first.
+        { do 2 f_equal. lia. }
+        rewrite /cf_hashmap_raw.
+        iExists (2 * vsval)%nat, (sval + 1)%nat, (2 * rval)%nat, _,(<[k:=#n]> img ++ replicate (vsval) #()).
+        rewrite /cf_hashfun_raw.
+        iDestruct "Hhash" as (?????) "(?&?&?&?&?&?&?&?&?&?&?& %Hprf)".
+        iFrame.
+        iSplit.
+        {
+          iPureIntro.
+          apply lt_INR.
+          lia.
+        }
+        iSplit.
+        {
+          iPureIntro.
+          rewrite app_length insert_length replicate_length.
+          lia.
+        }
+        iSplit.
+        {
+          iExists _,_,s0,_,_.
+          rewrite Heq.
+          iFrame.
+          iSplit.
+          { iPureIntro. rewrite mult_INR /=. lra. }
+          done.
+        }
+        iPureIntro.
+        destruct Hprf as (Hcf & Himg). split; [| split; [|split]].
+        * rewrite /filter_units.
+          simpl.
+          rewrite filter_app.
+          rewrite list_filter_insert_True; auto.
+          2:{ rewrite Hlen //. }
+          rewrite union_comm.
+          rewrite elements_union_singleton /=; last first.
+          {
+            intros H.
+            assert (#n ∈ filter_units img) as H2.
+            {
+              rewrite Hperm.
+              apply (elem_of_list_fmap).
+              eexists; split; eauto.
+              set_solver.
+            }
+            rewrite /filter_units in H2.
+            apply elem_of_list_filter in H2 as (H3 & H4).
+            apply elem_of_list_lookup_1 in H4 as (i & Hi).
+            apply HimgN in Hi. simplify_eq.
+          }
+          (* TODO: Move outside *)
+          assert (forall N, filter (λ v : val, v ≠ #()) (replicate N #()) = []) as ->.
+          {
+            induction N.
+            - simpl.
+              rewrite filter_nil //.
+            - simpl.
+              rewrite filter_cons /=.
+              apply IHN.
+          }
+          rewrite app_nil_r.
+          by apply perm_skip.
+
+        * intros i v. split; intros H.
+          ** destruct (decide (k = i)) as [-> | Hneqki].
+             *** rewrite lookup_app_l; last first.
+                 { rewrite insert_length. apply INR_lt. rewrite Hlen //. }
+                 rewrite list_lookup_insert; [ | apply INR_lt; rewrite Hlen // ].
+                 destruct (decide (n = v)) as [-> | Hneqnv]; auto.
+                 rewrite lookup_insert_ne in H; auto.
+                 exfalso. apply Hkimg.
+                 by eapply elem_of_map_img_2.
+             *** destruct (decide (n = v)) as [-> | Hneqnv]; auto.
+                 **** rewrite lookup_insert in H.
+                      inversion H; done.
+                 **** rewrite lookup_insert_ne in H; auto.
+                      rewrite lookup_app_l; last first.
+                      {
+                       rewrite insert_length. apply INR_lt.
+                       rewrite /is_bounded_prf in Hprf_pre.
+                       destruct Hprf_pre as (H3 & H4).
+                       rewrite Hlen.
+                       apply H4.
+                       apply elem_of_map_img; eauto.
+                     }
+                     rewrite list_lookup_insert_ne; auto.
+                     by apply HimgN.
+
+          ** destruct (decide (n = v)) as [-> | Hneqnv].
+             *** rewrite lookup_insert.
+                 destruct (decide (k = i)) as [-> | Hneqki]; auto.
+                 assert ((i < length img \/ length img <= i)%nat) as [?|?] by lia.
+                 **** rewrite lookup_app_l in H; [ | rewrite insert_length // ].
+                      rewrite list_lookup_insert_ne in H; auto.
+                      exfalso. apply Hkimg.
+                      set_solver.
+                 **** rewrite lookup_app_r in H; [ | rewrite insert_length // ].
+                      rewrite lookup_replicate in H.
+                      destruct H as (?&?).
+                      simplify_eq.
+
+             *** rewrite lookup_insert_ne; auto.
+                 apply HimgN.
+                 assert ((i < length img \/ length img <= i)%nat) as [?|?] by lia.
+                 **** rewrite lookup_app_l in H; [ | rewrite insert_length // ].
+                      destruct (decide (k = i)) as [-> | Hneqki]; auto.
+                      ***** rewrite list_lookup_insert in H; [inversion H; simplify_eq | ].
+                      rewrite Hlen. apply INR_lt; auto.
+                      ***** rewrite list_lookup_insert_ne in H; auto.
+                 **** rewrite lookup_app_r in H; [ | rewrite insert_length // ].
+                      rewrite lookup_replicate in H.
+                      destruct H as (?&?).
+                      simplify_eq.
+
+        * intros i Hi Hiimg.
+          destruct (decide (k = i)) as [-> | Hneqki].
+          ** exfalso.
+             apply Hiimg.
+             eapply elem_of_map_img.
+             exists n. rewrite lookup_insert //.
+          ** assert ((i < length img \/ length img <= i)%nat) as [?|?] by lia.
+             *** rewrite lookup_app_l; [ | rewrite insert_length // ].
+                 rewrite list_lookup_insert_ne; eauto.
+                 apply HimgU; auto.
+                 { apply lt_INR. lia. }
+                 intro Him.
+                 apply Hiimg.
+                 rewrite map_img_insert_notin; auto.
+                 set_solver.
+             *** rewrite lookup_app_r; [ | rewrite insert_length // ].
+                 rewrite lookup_replicate; split; auto.
+                 rewrite insert_length -Hlen.
+                 apply INR_lt in Hi.
+                 lia.
+        * rewrite dom_insert_L.
+          rewrite Hdom. set_solver.
+ Qed.
+
+
+End coll_free_hashmap.
